new/proof/io.v
@@ -9,4 +9,30 @@ Local Set Default Proof Using "All".
 #[global] Instance : IsPkgInit (iProp Σ) io := define_is_pkg_init True%I.
 #[global] Instance : GetIsPkgInitWf (iProp Σ) io := build_get_is_pkg_init_wf.
 
+Lemma wp_blackHolePool_init :
+  {{{ is_pkg_init sync }}}
+    io.blackHolePool'init #()
+  {{{ RET #(); True }}}.
+Proof.
+Admitted.
+
+Lemma wp_initialize' get_is_pkg_init :
+  get_is_pkg_init_prop io get_is_pkg_init →
+  {{{ own_initializing get_is_pkg_init }}}
+    io.initialize' #()
+  {{{ RET #(); own_initializing get_is_pkg_init ∗ is_pkg_init io }}}.
+Proof.
+  intros Hinit. wp_start as "Hown".
+  wp_apply (wp_package_init with "[$Hown] HΦ").
+  { destruct Hinit as (-> & ?); done. }
+  iIntros "Hown". wp_auto.
+  repeat wp_apply wp_GlobalAlloc as "?".
+  wp_apply (sync.wp_initialize' with "[$Hown]") as "(Hown & #?)"; first naive_solver.
+  wp_apply (errors.wp_initialize' with "[$Hown]") as "(Hown & #?)"; first naive_solver.
+  repeat wp_apply wp_New as "% _".
+  wp_apply wp_blackHolePool_init.
+  wp_apply wp_New as "% _".
+  iEval (rewrite is_pkg_init_unfold /=). iFrame "∗#". done.
+Qed.
+
 End wps.
