new/proof/slices_proof/slices_init.v
@@ -1,6 +1,7 @@
 From New.generatedproof Require Import slices.
 From New.proof Require Import proof_prelude.
 
+Module slices.
 Section proof.
 Context `{hG: heapGS Σ, !ffi_semantics _ _}.
 Context {sem : go.Semantics} {package_sem : slices.Assumptions}.
@@ -8,4 +9,19 @@ Collection W := sem + package_sem.
 
 #[global] Instance : IsPkgInit (iProp Σ) slices := define_is_pkg_init True%I.
 #[global] Instance : GetIsPkgInitWf (iProp Σ) slices := build_get_is_pkg_init_wf.
+
+Lemma wp_initialize' get_is_pkg_init :
+  get_is_pkg_init_prop slices get_is_pkg_init →
+  {{{ own_initializing get_is_pkg_init }}}
+    slices.initialize' #()
+  {{{ RET #(); own_initializing get_is_pkg_init ∗ is_pkg_init slices }}}.
+Proof using W.
+  intros Hinit. wp_start as "Hown".
+  wp_apply (wp_package_init with "[$Hown] HΦ").
+  { destruct Hinit as (-> & ?); done. }
+  iIntros "Hown". wp_auto.
+  iEval (rewrite is_pkg_init_unfold /=). iFrame "∗#". done.
+Qed.
+
 End proof.
+End slices.
